subst_ctx lemmas admitted

label-free/Substitution.v
@@ -5,557 +5,111 @@ Require Import List.
 
 Open Scope label_free_is5_scope.
 
-Definition var_from (w: ctx_LF):=
-match w with
-| fctx w0 => \{w0}
-| bctx _ => \{}
-end.
+Global Reserved Notation " [ M // v ] N " (at level 5).
+Global Reserved Notation " {{ w1 // w2 }} N " (at level 5).
 
 (* Term substitution *)
 
-(* We want to substitute M for nth hyp. in term N0 when the context is ctx.
-   We also know, that current context isn't ctx. *)
-Fixpoint subst_t_outer (M0: te_LF) (n: nat) (ctx: ctx_LF) (N0: te_LF) :=
+Fixpoint subst_t (M0: te_LF) (v0: var_LF) (N0: te_LF) :=
 match N0 with
-| hyp_LF n => 
-    hyp_LF n
+| hyp_LF v => 
+    if (eq_var_LF_dec v v0) then M0 else N0
 | lam_LF A M => 
-    lam_LF A (subst_t_outer M0 n ctx M)
+    lam_LF A ([M0 // var_succ v0] M) 
 | appl_LF M N => 
-    appl_LF (subst_t_outer M0 n ctx M) (subst_t_outer M0 n ctx N)
+    appl_LF ([M0//v0]M) ([M0//v0]N)
 | box_LF M => 
-    box_LF (subst_t_outer M0 n ctx M)
-| unbox_fetch_LF w M => 
-  let M' := If (ctx = w) then subst_t_inner M0 n M ctx
-            else subst_t_outer M0 n ctx M in
-    unbox_fetch_LF w M'
-| get_here_LF w M =>
-  let M' := If (ctx = w) then subst_t_inner M0 n M ctx
-            else subst_t_outer M0 n ctx M in
-    get_here_LF w M'        
-| letdia_get_LF w M N =>
-  let M' := If (ctx = w) then subst_t_inner M0 n M ctx
-            else subst_t_outer M0 n ctx M in
-  let N' := subst_t_outer M0 n ctx N in
-    letdia_get_LF w M' N'
-end
-(* Current context is exactly the context in which we want to do susbtitution *)
-with subst_t_inner (M0: te_LF) (n: nat) (N0: te_LF) (curr: ctx_LF) {struct N0} :=
-match N0 with
-| hyp_LF m => 
-    if (eq_nat_dec m n) then M0 else hyp_LF m
-| lam_LF A M => 
-    lam_LF A (subst_t_inner M0 (S n) M curr)
-| appl_LF M N => 
-    appl_LF (subst_t_inner M0 n M curr) (subst_t_inner M0 n N curr)
-| box_LF M =>
-    box_LF (subst_t_outer M0 n curr M)
+    box_LF ([M0//v0]M)
 | unbox_fetch_LF w M =>
-  let M' := If (curr = w) then subst_t_inner M0 n M curr
-            else subst_t_outer M0 n curr M in
-    unbox_fetch_LF w M'
+    unbox_fetch_LF w ([M0//v0]M)
 | get_here_LF w M =>
-  let M' := If (curr = w) then subst_t_inner M0 n M curr
-            else subst_t_outer M0 n curr M in
-    get_here_LF w M'
+    get_here_LF w ([M0//v0]M)
 | letdia_get_LF w M N =>
-  let M' := If (curr = w) then subst_t_inner M0 n M curr
-            else subst_t_outer M0 n curr M in
-  let N' := subst_t_inner M0 n N curr in
-    letdia_get_LF w M' N'
-end.
+    letdia_get_LF w ([M0//v0]M) ([M0//var_succ v0]N)
+end
+where " [ M // v ] N " := (subst_t M v N) : label_free_is5_scope.
 
-Definition subst_t M n ctx N curr :=
-  If ctx = curr then (subst_t_inner M n N ctx) 
-  else (subst_t_outer M n ctx N). 
+Definition open_var (M: te_LF) (t: te_LF) := subst_t t (bvar 0) M.
+Notation " M '^t^' t " := (open_var M t) (at level 5) : label_free_is5_scope.
 
-Notation " [ M // n | ctx ] [ N | curr ] " := 
-  (subst_t M n ctx N curr) (at level 5) : label_free_is5_scope.
-
-Fixpoint subst_list L n N subst_ctx curr_ctx :=
-match L with
-| nil => N
-| M :: L' => [M//n | subst_ctx] 
-             [subst_list L' (S n) N subst_ctx curr_ctx | curr_ctx]
-end.
 
 (* Context substitution *)
 
-Definition recalc_simpl_ctx (ctx:ctx_LF) : ctx_LF :=
-  match ctx with
-    | fctx _ => ctx
-    | bctx n => bctx (S n)
-end.
-
-Definition recalculate_ctx (ctx1: ctx_LF) (ctx2: ctx_LF) : prod ctx_LF ctx_LF :=
-  (recalc_simpl_ctx ctx1, recalc_simpl_ctx ctx2).
-
-(* We want to substitute ctx1 for every occ. of ctx2; our current context is
-   curr. *)
-(* In subst_ctx_outer it is assumed that current context is neither ctx1
-   nor ctx2 *)
-Fixpoint subst_ctx_outer (M0 : te_LF) (ctx1: ctx_LF) (ctx2: ctx_LF)
-                         (len_old: nat) (d_new: nat):=
+Fixpoint subst_ctx (M0 : te_LF) (ctx1: ctx_LF) (ctx2: ctx_LF) := 
 match M0 with 
 | hyp_LF n => hyp_LF n
-
-| lam_LF A M => lam_LF A (subst_ctx_outer M ctx1 ctx2 len_old d_new)
-
-| appl_LF M N => appl_LF (subst_ctx_outer M ctx1 ctx2 len_old d_new) 
-                         (subst_ctx_outer N ctx1 ctx2 len_old d_new)
-
-| box_LF M => 
-  let (ctx1', ctx2') := recalculate_ctx ctx1 ctx2 in 
-    box_LF (subst_ctx_outer M ctx1' ctx2' len_old d_new)
-
-| unbox_fetch_LF w M => 
-  let M' := If (w = ctx1) then subst_ctx_new M ctx1 ctx2 len_old d_new 
-            else If (w = ctx2) then subst_ctx_old M ctx1 ctx2 len_old d_new
-            else subst_ctx_outer M ctx1 ctx2 len_old d_new in
-  unbox_fetch_LF w M'
-
-| get_here_LF w M =>
-  let M' := If (w = ctx1) then subst_ctx_new M ctx1 ctx2 len_old d_new
-            else If (w = ctx2) then subst_ctx_old M ctx1 ctx2 len_old d_new
-            else subst_ctx_outer M ctx1 ctx2 len_old d_new in
-  get_here_LF w M'
-
-| letdia_get_LF w M N =>
-  let (ctx1', ctx2') := recalculate_ctx ctx1 ctx2 in
-  let M' := If (w = ctx1) then subst_ctx_new M ctx1 ctx2 len_old d_new
-            else If (w = ctx2) then subst_ctx_old M ctx1 ctx2 len_old d_new
-            else subst_ctx_outer M ctx1 ctx2 len_old d_new in
-  let N' := subst_ctx_outer N ctx1' ctx2' len_old d_new in
-  letdia_get_LF w M' N'
-end
-
-(* In subst_ctx_old we assume that current context was ctx2 *)
-with subst_ctx_old (M0 : te_LF) (ctx1: ctx_LF) (ctx2: ctx_LF) (len_old: nat) (d_new : nat):=
-match M0 with 
-| hyp_LF n => hyp_LF n
-
-| lam_LF A M =>
-  let len_old' := match ctx2 with (* ? *)
-                  | bctx _ => len_old
-                  | fctx _ => S len_old
-                  end in
-  lam_LF A (subst_ctx_old M ctx1 ctx2 len_old' d_new)
-
-| appl_LF M N => appl_LF (subst_ctx_old M ctx1 ctx2 len_old d_new) 
-                         (subst_ctx_old N ctx1 ctx2 len_old d_new)
-
-| box_LF M =>
-  let (ctx1', ctx2') := recalculate_ctx ctx1 ctx2 in     
-    box_LF (subst_ctx_outer M ctx1' ctx2' len_old d_new)
-
+| lam_LF A M => lam_LF A ({{ctx1//ctx2}}M)
+| appl_LF M N => appl_LF ({{ctx1//ctx2}}M) ({{ctx1//ctx2}}N)
+| box_LF M =>  
+  box_LF ({{ ctx_succ ctx1 // ctx_succ ctx2 }} M)
 | unbox_fetch_LF w M =>
-  let M' := If (w = ctx1) then subst_ctx_new M ctx1 ctx2 len_old d_new
-            else If (w = ctx2) then subst_ctx_old M ctx1 ctx2 len_old d_new
-            else subst_ctx_outer M ctx1 ctx2 len_old d_new in
-  unbox_fetch_LF w M'
-
+  let w' := If w = ctx2 then ctx1 else w in
+    unbox_fetch_LF w' ({{ctx1//ctx2}} M)
 | get_here_LF w M =>
-  let M' := If (w = ctx1) then subst_ctx_new M ctx1 ctx2 len_old d_new
-            else If (w = ctx2) then subst_ctx_old M ctx1 ctx2 len_old d_new
-            else subst_ctx_outer M ctx1 ctx2 len_old d_new in
-  get_here_LF w M'
-
+  let w' := If w = ctx2 then ctx1 else w in
+    get_here_LF w' ({{ctx1//ctx2}}M)
 | letdia_get_LF w M N =>
-  let (ctx1', ctx2') := recalculate_ctx ctx1 ctx2 in
-  let M' := If (w = ctx1) then subst_ctx_new M ctx1 ctx2 len_old d_new
-            else If (w = ctx2) then subst_ctx_old M ctx1 ctx2 len_old d_new
-            else subst_ctx_outer M ctx1 ctx2 len_old d_new in
-  let N' := subst_ctx_old N ctx1' ctx2' len_old d_new in
-  letdia_get_LF w M' N'
+  let w' := If w = ctx2 then ctx1 else w in
+    letdia_get_LF w' ({{ctx1//ctx2}} M) ({{ctx_succ ctx1 // ctx_succ ctx2}} N)
 end
+where " {{ w1 // w2 }} M " := (subst_ctx M w1 w2) : label_free_is5_scope.
 
-(* In subst_ctx_new we assume that current context is ctx1 *)
-with subst_ctx_new (M0 : te_LF) (ctx1: ctx_LF) (ctx2: ctx_LF) (len_old: nat) (d_new: nat) :=
-match M0 with 
-(* It is assumed that when ctx2 = bctx _, then len_old is 0 *)
-| hyp_LF n => If n < d_new then hyp_LF n else hyp_LF (len_old + n)
-
-| lam_LF A M =>  lam_LF A (subst_ctx_new M ctx1 ctx2 len_old (S d_new))
-
-| appl_LF M N => appl_LF (subst_ctx_new M ctx1 ctx2 len_old d_new) 
-                         (subst_ctx_new N ctx1 ctx2 len_old d_new)
-
-| box_LF M =>
-  let (ctx1', ctx2') := recalculate_ctx ctx1 ctx2 in 
-    box_LF (subst_ctx_outer M ctx1' ctx2' len_old d_new)
-
-| unbox_fetch_LF w M =>
-  let M' := If (w = ctx1) then subst_ctx_new M ctx1 ctx2 len_old d_new
-            else If (w = ctx2) then subst_ctx_old M ctx1 ctx2 len_old d_new
-            else subst_ctx_outer M ctx1 ctx2 len_old d_new in
-  unbox_fetch_LF w M'
-
-| get_here_LF w M =>
-  let M' := If (w = ctx1) then subst_ctx_new M ctx1 ctx2 len_old d_new
-            else If (w = ctx2) then subst_ctx_old M ctx1 ctx2 len_old d_new
-            else subst_ctx_outer M ctx1 ctx2 len_old d_new in
-  get_here_LF w M'
-
-| letdia_get_LF w M N =>
-  let (ctx1', ctx2') := recalculate_ctx ctx1 ctx2 in
-  let M' := If (w = ctx1) then subst_ctx_new M ctx1 ctx2 len_old d_new
-            else If (w = ctx2) then subst_ctx_old M ctx1 ctx2 len_old d_new
-            else subst_ctx_outer M ctx1 ctx2 len_old d_new in
-  let N' := subst_ctx_old N ctx1' ctx2' len_old d_new in
-  letdia_get_LF w M' N'
-end.
-
-Definition subst_ctx M c1 c2 curr len_old d_new :=
-If c1 = c2 then M
-else
-  If curr = c1 then
-    subst_ctx_new M c1 c2 len_old d_new
-  else
-    If curr = c2 then
-      subst_ctx_old M c1 c2 len_old d_new
-    else
-      subst_ctx_outer M c1 c2 len_old d_new.
-
-Notation " {{ c1 // c2 }} [ M | curr , m , d ] " := 
-  (subst_ctx M c1 c2 curr m d) (at level 5) : label_free_is5_scope.
-
-Definition open_ctx M ctx curr := subst_ctx M ctx (bctx 0) curr 0 0.
-
-Notation " M ^^ [ w | w' ] " := (open_ctx M w w') (at level 10) : label_free_is5_scope.
+Definition open_ctx M ctx := subst_ctx M ctx (bctx 0).
+Notation " M ^w^ w  " := (open_ctx M w) (at level 10) : label_free_is5_scope.
 
 
 Section Lemmas.
 
-Lemma subst_t__inner:
-forall M k N w,
-  subst_t_inner M k N w = [M//k | w] [N | w].
-intros;
-unfold subst_t;
-case_if;
-reflexivity.
-Qed.
-
-Lemma subst_t__outer:
-forall M k N w w'
-  (Neq: w <> w'),
-  subst_t_outer M k w N = [M//k | w] [N | w'].
-intros; unfold subst_t;
-case_if; reflexivity.
-Qed.
-
-Lemma subst_ctx__old:
-forall M c1 c2 len_old d_new
-  (Neq: c1 <> c2),
-  subst_ctx_old M c1 c2 len_old d_new  = {{ c1 // c2 }} [M | c2, len_old, d_new].
-intros;
-unfold subst_ctx;
-repeat case_if;
-reflexivity.
-Qed.
-
-Lemma subst_ctx__new:
-forall M c1 c2 len_old d_new
-  (Neq: c1 <> c2),
-  subst_ctx_new M c1 c2 len_old d_new = {{ c1 // c2 }} [M | c1, len_old, d_new].
-intros;
-unfold subst_ctx;
-repeat case_if;
-reflexivity.
-Qed.
-
-Lemma subst_ctx__outer:
-forall M c1 c2 curr len_old d_new
-  (Neq: c1 <> c2)
-  (Neq': c1 <> curr)
-  (Neq'': c2 <> curr),
-  subst_ctx_outer M c1 c2 len_old d_new = {{ c1 // c2 }} [M | curr, len_old, d_new].
-intros;
-unfold subst_ctx;
-repeat case_if;
-reflexivity.
-Qed.
-
-Ltac try_rewrite_subst :=
-try repeat rewrite subst_t__inner;
-try repeat rewrite subst_ctx__new;
-try repeat rewrite subst_ctx__old.
-
-Lemma no_changes_subst_w_id_d_new:
-forall w w' w0 n k  M,
-  {{w//w'}}[M | w0, n, k] = M ->
-  {{w//w'}}[M | w0, n, S k] = M.
-Admitted.
-Hint Resolve no_changes_subst_w_id_d_new.
-
-Lemma no_unbound_worlds_LF_subst_w_id:
-forall M n
+Lemma no_unbound_worlds_LF_subst_ctx_id:
+forall M n w
   (H_unbound: unbound_worlds n M = nil),
-  forall w w0 k, {{ w // bctx n }} [M | w0, 0, k] = M.
-induction M; intros; unfold subst_ctx.
-(* hyp *)
-repeat case_if; simpl; try reflexivity;
-case_if; reflexivity.
-(* lam *)
-unfold subst_ctx;
-simpl in H_unbound.
-repeat case_if; subst; eauto;
-simpl; try_rewrite_subst; eauto;
-try erewrite IHM with (k:=S k); eauto;
-try erewrite IHM with (k:=k); eauto.
-rewrite subst_ctx__outer with (curr:=w0); auto;
-try erewrite IHM with (k:=k); eauto.
-(* appl *)
-unfold subst_ctx in *;
-simpl in H_unbound;
-apply app_eq_nil in H_unbound;
-destruct H_unbound as (H_Un1, H_Un2);
-eapply IHM1 with (w:=w) (w0:=w0) (k:=k) in H_Un1;
-eapply IHM2 with (w:=w) (w0:=w0) (k:=k) in H_Un2;
-repeat case_if; simpl;
-try (rewrite H_Un1; rewrite H_Un2); reflexivity.
-(* box *)
-inversion H_unbound; subst;
-apply IHM with (w:=w) (w0:=w0) (k:=k) in H0;
-repeat case_if; simpl; try subst; auto;
-unfold recalc_simpl_ctx;
-assert (exists w0, w0 \notin free_worlds_LF M \u var_from w) by
-  (exists (var_gen (free_worlds_LF M \u var_from w)); apply var_gen_spec).
-destruct H2 as (w_fresh);
-rewrite notin_union in H2; destruct H2;
-rewrite subst_ctx__outer with (curr := fctx w_fresh);
-try rewrite IHM; eauto; try discriminate;
-destruct w; simpl in H3;
-try (intro nn; inversion nn; subst n0; elim H; reflexivity);
-try discriminate;
-rewrite notin_singleton in H3;
-intro nn; inversion nn; subst v; elim H3; reflexivity.
+  {{ w // bctx n }} M = M.
+Admitted.
 
-destruct H3 as (w_fresh);
-rewrite notin_union in H3; destruct H3;
-rewrite subst_ctx__outer with (curr := fctx w_fresh);
-try rewrite IHM; eauto; try discriminate;
-destruct w; simpl in H4;
-try (intro nn; inversion nn; subst n0; elim H; reflexivity);
-try discriminate;
-rewrite notin_singleton in H4;
-intro nn; inversion nn; subst v; elim H4; reflexivity.
-
-destruct H3 as (w_fresh);
-rewrite notin_union in H3; destruct H3;
-rewrite subst_ctx__outer with (curr := fctx w_fresh);
-try rewrite IHM; eauto; try discriminate;
-destruct w; simpl in H4;
-try (intro nn; inversion nn; subst n0; elim H; reflexivity);
-try discriminate;
-rewrite notin_singleton in H4;
-intro nn; inversion nn; subst v; elim H4; reflexivity.
-(* unbox_fetch *)
-inversion H_unbound; destruct c; simpl; try discriminate;
-assert (exists w0, w0 \notin free_worlds_LF M \u var_from w) by
-  (exists (var_gen (free_worlds_LF M \u var_from w)); apply var_gen_spec);
-destruct H as (w_fresh);
-repeat case_if; simpl;
-try rewrite subst_ctx__old;
-try rewrite subst_ctx__new;
-try rewrite subst_ctx__outer with (curr:=fctx w_fresh);
-try discriminate;
-try rewrite IHM; 
-eauto;
-rewrite notin_union in H; unfold var_from in *;
-destruct w;
-try rewrite notin_singleton in H;
-destruct H; try discriminate;
-intro nn; inversion nn; subst w_fresh. 
-elim H5; reflexivity.
-elim H6; reflexivity.
-elim H6; reflexivity.
-(* get_here *)
-inversion H_unbound; destruct c; simpl; try discriminate;
-assert (exists w0, w0 \notin free_worlds_LF M \u var_from w) by
-  (exists (var_gen (free_worlds_LF M \u var_from w)); apply var_gen_spec);
-destruct H as (w_fresh);
-rewrite notin_union in H; unfold var_from in *;
-destruct w;
-try rewrite notin_singleton in H; destruct H;
-repeat case_if; simpl;
-try rewrite subst_ctx__old;
-try rewrite subst_ctx__new;
-try rewrite subst_ctx__outer with (curr := fctx w_fresh);
-try discriminate;
-try rewrite IHM; 
-eauto;
-intro nn; inversion nn; subst w_fresh;
-elim H1; reflexivity.
-
-(* letdia_get *)
-inversion H_unbound; destruct c; simpl; try discriminate;
-apply app_eq_nil in H0; destruct H0;
-assert (exists w0, w0 \notin free_worlds_LF M1 \u free_worlds_LF M2 \u var_from w) by
-  (exists (var_gen (free_worlds_LF M1 \u free_worlds_LF M2 \u var_from w)); apply var_gen_spec);
-destruct H1 as (w_fresh);
-repeat rewrite notin_union in H1; unfold var_from in *;
-destruct H1; destruct H2; destruct w;
-repeat rewrite notin_singleton in H3; 
-repeat case_if; simpl;
-eauto;
-unfold recalc_simpl_ctx in *;
-try destruct w0;
-try repeat rewrite subst_ctx__old;
-try repeat rewrite subst_ctx__new;
-try repeat rewrite subst_ctx__outer with (curr := fctx w_fresh);
-try discriminate;
-try rewrite IHM1;
-try rewrite IHM2; 
-eauto;
-try inversion H5;
-try (intro nn; inversion nn; subst; elim H4; reflexivity);
-try (intro nn; inversion nn; subst; elim H3; reflexivity).
-Qed.
-
-Lemma closed_ctx_subst_id:
-forall M w n curr l
+Lemma closed_ctx_subst_ctx_id:
+forall M w n
   (H_lc: lc_w_n_LF M n),
-  {{w // bctx n}} [ M | curr, 0, l] = M.
-intros;
-apply no_unbound_worlds_LF_subst_w_id;
-apply closed_no_unbound_worlds;
-assumption.
-Qed.
+  {{w // bctx n}} M  = M.
+Admitted.
+
+Lemma subst_ctx_comm:
+forall M w w' w'' n
+  (Neq: w'' <> w),
+  {{fctx w'//fctx w''}}({{fctx w//bctx n}}M) = 
+  {{fctx w//bctx n}}({{fctx w'//fctx w''}}M).
+Admitted.
+
+Lemma subst_ctx_id:
+forall M w n
+  (HT: w \notin free_worlds_LF M),
+  {{bctx n//fctx w}}({{fctx w//bctx n}}M) = M.
+Admitted.
+
+Lemma subst_ctx_neutral_free:
+forall M w w' w0
+  (HT: w0 \notin free_worlds_LF M),
+  {{w//fctx w0}}({{fctx w0// w'}}M) = {{w//w'}}M.
+Admitted.
+
+Lemma subst_ctx_neutral_bound:
+forall M w w' n
+  (HT: lc_w_n_LF M n),
+  {{w//bctx n}}({{bctx n// w'}}M) = {{w//w'}}M.
+Admitted.
+
+Lemma closed_ctx_step_opening:
+forall M n w
+  (HT: lc_w_n_LF M (S n)),
+  lc_w_n_LF ({{fctx w//bctx n}}M) n.
+Admitted.
+
 
 Lemma subst_order_irrelevant:
-forall N w w' M n m w0 w1 l
+forall N w M v m
   (HT_M: lc_w_LF M),
-    [M // n | w0] [{{w1 // bctx m}}[N | w, 0, l] | w'] = 
-    {{w1 // bctx m}}[ [M // n | w0] [N | w'] | w, 0, l].
-induction N; unfold subst_t; unfold subst_ctx; intros;
-remember (var_from w \u var_from w' \u var_from w0 \u var_from w1) as known_worlds;
-assert (exists w', w' \notin known_worlds) by
-  (exists (var_gen known_worlds); eapply var_gen_spec);
-destruct H as (w_fresh); subst; repeat rewrite notin_union in *;
-repeat rewrite notin_singleton in *;
-destruct H; destruct H0; destruct H1.
-(* hyp *)
-repeat (case_if; simpl in * ); subst; simpl in *; try reflexivity;
-try_rewrite_subst; auto;
-try rewrite subst_ctx__outer with (curr := fctx w_fresh); eauto;
-try rewrite closed_ctx_subst_id; auto;
-try discriminate;
-try (intro nn; inversion nn; subst;
-     simpl in H2; rewrite notin_singleton in H2;
-     elim H2; reflexivity);
-unfold lc_w_LF in HT_M; replace m with (0+m) by omega;
-apply closed_w_addition; assumption.
-(* lam *)
-repeat case_if; subst; simpl in *; eauto;
-try_rewrite_subst; auto;
-repeat erewrite subst_t__outer; eauto;
-repeat rewrite subst_ctx__outer with (curr := fctx w_fresh); simpl;
-eauto;
-try rewrite IHN; eauto;
-try destruct w1;
-try discriminate;
-try (simpl in *; rewrite notin_singleton in H2; intro nn;
-     inversion nn; subst; elim H2; reflexivity).
-(* appl *)
-repeat (case_if; simpl in * ); subst; simpl in *;
-try_rewrite_subst; simpl;
-try rewrite IHN1; try rewrite IHN2; auto;
-repeat erewrite subst_t__outer; eauto;
-repeat rewrite subst_ctx__outer with (curr := fctx w_fresh); eauto;
-try (erewrite IHN1; try erewrite IHN2; eauto);
-try destruct w1;
-try discriminate;
-try (simpl in *; rewrite notin_singleton in *; intro nn;
-  inversion nn; subst);
-try elim H2; reflexivity.
-(* box *)
-repeat (case_if; simpl in * ); subst; simpl in *;
-try_rewrite_subst; simpl;
-repeat rewrite subst_t__outer with (w':= fctx w_fresh); eauto;
-repeat rewrite subst_ctx__outer with (curr := fctx w_fresh); eauto;
-try rewrite IHN; auto;
-try destruct w0;
-try destruct w1;
-try destruct w;
-try destruct w';
-try discriminate;
-try (simpl in *; rewrite notin_singleton in *; simpl; intro nn;
-     inversion nn; subst);
-try (elim H; reflexivity);
-try (elim H0; reflexivity);
-try (elim H1; reflexivity);
-try (elim H2; reflexivity);
-try (elim H3; reflexivity);
-try (simpl; intro nn; inversion nn; subst);
-try (elim H4; reflexivity). 
-(* unbox_fetch *)
-repeat (case_if; simpl in * ); subst; simpl in *;
-try_rewrite_subst; simpl;
-repeat rewrite subst_t__outer with (w':= fctx w_fresh); eauto;
-repeat rewrite subst_ctx__outer with (curr := fctx w_fresh); eauto;
-try rewrite IHN; auto;
-try destruct w;
-try destruct w';
-try destruct w0;
-try destruct w1;
-try discriminate;
-try (simpl in *; rewrite notin_singleton in *; intro nn;
-  inversion nn; subst);
-try (elim H; reflexivity);
-try (elim H0; reflexivity);
-try (elim H1; reflexivity);
-try (elim H2; reflexivity);
-try (elim H3; reflexivity);
-try (elim H4; reflexivity);
-try (elim H5; reflexivity);
-try (elim H6; reflexivity).
-(* get_here *)
-repeat (case_if; simpl in * ); subst; simpl in *;
-try_rewrite_subst; simpl;
-repeat rewrite subst_t__outer with (w':= fctx w_fresh); eauto;
-repeat rewrite subst_ctx__outer with (curr := fctx w_fresh); eauto;
-try rewrite IHN; auto;
-try destruct w;
-try destruct w';
-try destruct w0;
-try destruct w1;
-try discriminate;
-try (simpl in *; rewrite notin_singleton in *; intro nn;
-  inversion nn; subst);
-try (elim H; reflexivity);
-try (elim H0; reflexivity);
-try (elim H1; reflexivity);
-try (elim H2; reflexivity);
-try (elim H3; reflexivity);
-try (elim H4; reflexivity);
-try (elim H5; reflexivity);
-try (elim H6; reflexivity).
-(* letdia_get *)
-repeat (case_if; simpl in * ); subst; simpl in *;
-try_rewrite_subst; simpl;
-repeat rewrite subst_t__outer with (w':= fctx w_fresh); eauto;
-repeat rewrite subst_ctx__outer with (curr := fctx w_fresh); eauto;
-try rewrite IHN1;
-try rewrite IHN2; auto;
-try destruct w;
-try destruct w';
-try destruct w0;
-try destruct w1;
-try discriminate;
-simpl;
-try (simpl in *; rewrite notin_singleton in *);
-try (intro nn; inversion nn; subst);
-try (elim H; reflexivity);
-try (elim H0; reflexivity);
-try (elim H1; reflexivity);
-try (elim H2; reflexivity);
-try (elim H3; reflexivity);
-try (elim H4; reflexivity);
-try (elim H5; reflexivity);
-try (elim H6; reflexivity);
-try (elim H7; reflexivity);
-simpl in H1; rewrite notin_singleton in H1; elim H1; reflexivity.
-Qed.
+    [M // v ] ({{w // bctx m}} N)  = 
+    {{w // bctx m}} ([M // v ] N). 
+Admitted.
 
 End Lemmas.
 
